Add compute valid token mask

ConstrainedDecodingFormalization/GrammarConstrainedDecoding.lean
@@ -7,8 +7,9 @@ variable { α : Type u } { Γ : Type u } { π : Type v } { σ : Type w } { σ0 :
 
 variable [ BEq π ] [ DecidableEq σ ] [DecidableEq Γ ] [ DecidableEq α ]
 
-def PreprocessParser (fst_comp : FSTComp α Γ σ0) (p : PDA Γ π σ) : 
-      (σ → σ0 → (List (Token (Ch α)) × List (List Γ))) := 
+abbrev PPTable (α σ σ0 Γ):= (σ → σ0 → (List (Token (Ch α)) × List (List Γ)))
+
+def PreprocessParser (fst_comp : FSTComp α Γ σ0) (p : PDA Γ π σ) : PPTable α σ σ0 Γ := 
   let (re, tist) := BuildInverseTokenSpannerTable fst_comp 
   fun qp =>
     let accepted := re.filter (λ s => (p.evalFrom (some (qp, [])) s).isSome)
@@ -21,4 +22,27 @@ def PreprocessParser (fst_comp : FSTComp α Γ σ0) (p : PDA Γ π σ) :
       let dependent_a := dependent_a.dedup
       (accepted_a, dependent_a)
 
+def ComputeValidTokenMask (P : PDA Γ π σ) (itst : List Γ → σ0 → (List (Token (Ch α)))) (table : PPTable α σ σ0 Γ) (qa : σ0) (qp : σ) (st : List π) : List (Token (Ch α)) := Id.run do
+  let mut accepted := (table qp qa).fst
+  for d in (table qp qa).snd do
+    if (P.evalFrom (some (qp, st)) d).isSome then 
+      accepted := accepted ++ (itst d qa)
+
+  accepted.dedup
+
+-- if in compute valid token mask, parser would accept it
+-- we want something a bit stronger than this, basically having to do with the
+-- assumption about all terminal sequences being realizable
+theorem accept_if_ComputedValidTokenMask (P : PDA Γ π σ) (fst_comp : FSTComp α Γ σ0) : 
+  ∀ st qa qp v, 
+    v ∈ (ComputeValidTokenMask P (BuildInverseTokenSpannerTable fst_comp).snd (PreprocessParser fst_comp P) qa qp st) →
+    -- jointly evaluating, it is still accepted
+    -- P.evalFrom qp st (all new symbols)
+    True
+  := by sorry
+
+-- if compute valid token mask rejects it, 
+-- the parser would reject it (now or in the future)
+-- so it must mean there is no way to get to an accepting state 
+theorem ComputedValidTokenMask_complete : 0 = 0 := by sorry
 
