ConstrainedDecodingFormalization.lean
@@ -6,6 +6,7 @@ import «ConstrainedDecodingFormalization».CFG
 import «ConstrainedDecodingFormalization».Automata
 import «ConstrainedDecodingFormalization».Vocabulary
 import «ConstrainedDecodingFormalization».ConstrainedDecoding
+import «ConstrainedDecodingFormalization».GrammarConstrainedDecoding
 import «ConstrainedDecodingFormalization».Checker
 import «ConstrainedDecodingFormalization».PDA
 import «ConstrainedDecodingFormalization».Language
